Clap/eDSLState/HashCons/EvalButActuallyGood.lean
@@ -1,0 +1,34 @@
+import Clap.eDSLState.HashCons.HashConsM
+
+namespace Clap.HashConsM
+
+abbrev ValueCache (p : ℕ) := Array (Option (ZMod p))
+
+def Barney {p} (Γ : VarStore p) (expr : CacheExpr p) (cache : ValueCache p) : Option (ZMod p) :=
+  match expr with
+  | .c k => .some k
+  | .v idx => Γ[idx]?
+  | .binary_op lhs rhs op =>
+    let op := match op with
+              | .add => (· + ·)
+              | .sub => (· - ·)
+              | .mul => (· * ·)
+    let lhs := cache[lhs]!
+    let rhs := cache[rhs]!
+    op <$> lhs <*> rhs
+
+def evalWithCache {p}
+  (varStore : VarStore p) (e : ExprRef) (cache : ValueCache p) (σ : HashConsSt p) : ValueCache p :=
+  if e < cache.size
+  then cache
+  else match σ[e]? with
+       | .none => cache
+       | .some expr => let val := Barney varStore expr cache
+                       evalWithCache varStore e (cache.push val) σ
+  termination_by (e + 1) - cache.size
+  decreasing_by grind
+ 
+def eval {p} (varStore : VarStore p) (e : ExprRef) (σ : HashConsSt p) : Option (ZMod p) :=
+  (evalWithCache varStore e #[] σ)[e]!
+
+end Clap.HashConsM
